Making progress on insert

total_order.dfy
@@ -1,5 +1,8 @@
+include "mathematics.dfy"
+  
 abstract module Total_Order {
-
+  import Mathematics
+    
 	type Element(!new,==)
 
 	predicate method lt(a: Element, b: Element)
@@ -14,6 +17,176 @@ abstract module Total_Order {
 		ensures forall a, b, c :: ltedef(a, b) && ltedef(b, c) ==> ltedef(a, c); // Transitive
 
 	predicate method ltedef(a: Element, b: Element)
+
+  function method Min(a: Element, b: Element) : Element
+  {
+    if lte(a, b) then a else b
+  }
+    
+  method SeqMinIndex(run: seq<Element>) returns (pos: int)
+    requires 0 < |run|;
+    ensures 0 <= pos < |run|;
+    ensures forall i :: 0 <= i < |run| ==> lte(run[pos], run[i]);
+  {
+    pos := 0;
+    var i := 1;
+    while i < |run|
+      invariant 0 <= i <= |run|;
+      invariant pos < i;
+      invariant forall j :: 0 <= j < i ==> lte(run[pos], run[j]);
+    {
+      if lt(run[i], run[pos]) {
+        pos := i;
+      }
+      i := i + 1;
+    }
+  }
+
+  method SeqMin(run: seq<Element>) returns (elt: Element)
+    requires 0 < |run|;
+    ensures elt in run;
+    ensures forall elt':: elt' in run ==> lte(elt, elt');
+  {
+    var index := SeqMinIndex(run);
+    elt := run[index];
+  }
+  
+  method SeqMaxIndex(run: seq<Element>) returns (pos: int)
+    requires 0 < |run|;
+    ensures 0 <= pos < |run|;
+    ensures forall i :: 0 <= i < |run| ==> lte(run[i], run[pos]);
+  {
+    pos := 0;
+    var i := 1;
+    while i < |run|
+      invariant 0 <= i <= |run|;
+      invariant pos < i;
+      invariant forall j :: 0 <= j < i ==> lte(run[j], run[pos]);
+    {
+      if lt(run[pos], run[i]) {
+        pos := i;
+      }
+      i := i + 1;
+    }
+  }
+
+  method SeqMax(run: seq<Element>) returns (elt: Element)
+    requires 0 < |run|;
+    ensures elt in run;
+    ensures forall elt':: elt' in run ==> lte(elt', elt);
+  {
+    var index := SeqMaxIndex(run);
+    elt := run[index];
+  }
+  
+  function method Max(a: Element, b: Element) : Element
+  {
+    if lte(a, b) then b else a
+  }
+    
+  predicate method IsSorted(run: seq<Element>) {
+    forall i, j :: 0 <= i <= j < |run| ==> lte(run[i], run[j])
+  }
+
+  method FindLargestLTE(run: seq<Element>, needle: Element) returns (pos: int)
+    requires IsSorted(run);
+    requires 0 < |run|;
+    ensures -1 <= pos < |run|;
+    ensures forall i :: 0 <= i <= pos ==> lte(run[i], needle);
+    ensures forall i :: pos < i < |run| ==> lt(needle, run[i]);
+  {
+    pos := -1;
+    while pos < |run|-1 && lte(run[pos + 1], needle)
+      invariant -1 <= pos < |run|;
+      invariant forall i :: 0 <= i <= pos ==> lte(run[i], needle);
+    {
+      pos := pos + 1;
+    }
+  }
+
+  method Merge(run1: seq<Element>, run2: seq<Element>) returns (result: array<Element>)
+    requires 0 < |run1|;
+    requires IsSorted(run1);
+    requires IsSorted(run2);
+    ensures multiset(result[..]) == multiset(run1) + multiset(run2);
+    ensures IsSorted(result[..]);
+  {
+    result := new Element[|run1| + |run2|](_ => run1[0]);
+    var i1 := 0;
+    var i2 := 0;
+    assert multiset(result[0..i1+i2]) == multiset(run1[0..i1]) + multiset(run2[0..i2]);
+    while i1 < |run1| || i2 < |run2|
+      invariant 0 <= i1 <= |run1|;
+      invariant 0 <= i2 <= |run2|;
+      invariant forall i, j :: 0 <= i < i1 + i2 && i1 <= j < |run1| ==> lte(result[i], run1[j]);
+      invariant forall i, j :: 0 <= i < i1 + i2 && i2 <= j < |run2| ==> lte(result[i], run2[j]);
+      invariant IsSorted(result[0..i1 + i2]);
+      invariant multiset(result[0..i1+i2]) == multiset(run1[0..i1]) + multiset(run2[0..i2]);
+      decreases |run1| + |run2| - i1 - i2;
+    {
+      if i1 < |run1| && i2 < |run2| {
+        if lte(run1[i1], run2[i2]) {
+          result[i1 + i2] := run1[i1];
+          i1 := i1 + 1;
+          assert run1[0..i1] == run1[0..i1-1] + run1[i1-1..i1]; // OBSERVE
+        } else {
+          result[i1 + i2] := run2[i2];
+          i2 := i2 + 1;
+          assert run2[0..i2] == run2[0..i2-1] + run2[i2-1..i2]; // OBSERVE
+        }
+      } else if i1 < |run1| {
+          result[i1 + i2] := run1[i1];
+          i1 := i1 + 1;
+          assert run1[0..i1] == run1[0..i1-1] + run1[i1-1..i1];
+      } else {
+          result[i1 + i2] := run2[i2];
+          i2 := i2 + 1;
+          assert run2[0..i2] == run2[0..i2-1] + run2[i2-1..i2];
+      }
+    }
+    assert result[..] == result[0..i1+i2]; // OBSERVE
+    assert run1 == run1[0..i1]; // OBSERVE
+    assert run2 == run2[0..i2]; // OBSERVE
+  }
+
+  method MergeSort(run: seq<Element>) returns (result: array<Element>)
+    ensures multiset(result[..]) == multiset(run);
+    ensures IsSorted(result[..]);
+  {
+    if |run| == 0 {
+      result := new Element[|run|];
+    } else if |run| <= 1 {
+      result := new Element[|run|](i => run[0]);
+    } else {
+      var i := |run| / 2;
+      assert |multiset(run[..i])| > 0; // OBSERVE
+      assert run == run[..i] + run[i..]; // OBSERVE
+      var a1 := MergeSort(run[..i]);
+      var a2 := MergeSort(run[i..]);
+      result :=  Merge(a1[..], a2[..]);
+    }
+  }
+
+  predicate SetAllLte(a: set<Element>, b: set<Element>) {
+    forall x, y :: x in a && y in b ==> lte(x, y)
+  }
+  
+  predicate SetAllLt(a: set<Element>, b: set<Element>) {
+    forall x, y :: x in a && y in b ==> lt(x, y)
+  }
+
+  lemma SetLtLteTransitivity(a: set<Element>, b: set<Element>, c: set<Element>)
+    requires SetAllLt(a, b);
+    requires SetAllLte(b, c);
+    requires |b| > 0;
+    ensures  SetAllLt(a, c);
+  {
+  }
+  
+  lemma SetAllLtImpliesDisjoint(a: set<Element>, b: set<Element>)
+    requires SetAllLt(a, b);
+    ensures a !! b;
+  {}
 }
 
 abstract module Bounded_Total_Order refines Total_Order {
