mathematics.dfy
@@ -15,4 +15,14 @@ module Mathematics {
 		else
 			a
 	}
+
+  function method Set<T>(ms: multiset<T>) : set<T>
+  {
+    set x : T | x in ms
+  }
+
+  function method ISet<T>(ms: set<T>) : iset<T>
+  {
+    iset x : T | x in ms
+  }
 }
